3/4 of inv_write case

proofs/inv_write.dfy
@@ -1,6 +1,14 @@
 datatype page = Node(data : int)
 datatype tlb_entry = Node(present : bool, readable : bool, writable : bool, ppn : int)
 
+function no_page_aliasing(tlb : map<int, tlb_entry>) : bool 
+{
+    forall vpn1, vpn2 :: vpn1 != vpn2 && 
+        vpn1 in tlb &&
+        vpn2 in tlb 
+        ==> tlb[vpn1].ppn != tlb[vpn2].ppn
+}
+
 // copies data from device to host
 method dma_read(vpn : int, 
                 host_mem : map<int, page>, host_tlb : map<int, tlb_entry>, 
@@ -12,6 +20,7 @@ method dma_read(vpn : int,
     // Our DMA transfer method also requires the vpn to be writeable
     requires vpn in host_tlb
     requires legal_vaddr(vpn, host_mem, host_tlb)
+    requires no_page_aliasing(host_tlb) && no_page_aliasing(device_tlb)
 
     // We are reading from the device, there should be data there
     requires(vpn_present(vpn, device_mem, device_tlb))
@@ -19,7 +28,14 @@ method dma_read(vpn : int,
     // Original host/device pages are untouched
     ensures no_side_effects(vpn, host_mem, host_tlb, new_host_mem, host_tlb)
     ensures valid_ppns(host_mem, host_tlb) ==> valid_ppns(new_host_mem, host_tlb)
-    ensures valid_memory(host_mem, host_tlb, device_mem, device_tlb) ==> valid_memory(new_host_mem, host_tlb, device_mem, device_tlb)
+    ensures valid_memory(host_mem, host_tlb, device_mem, device_tlb) && vpn !in host_tlb ==> 
+            valid_memory(new_host_mem, host_tlb, device_mem, device_tlb)
+    ensures valid_memory(host_mem, host_tlb, device_mem, device_tlb) && 
+            !ppn_writable(vpn, device_mem, device_tlb) && 
+            host_tlb[vpn].ppn in new_host_mem && 
+            new_host_mem[host_tlb[vpn].ppn] == device_mem[device_tlb[vpn].ppn] ==> 
+            valid_memory(new_host_mem, host_tlb, device_mem, device_tlb)
+    // ensures valid_memory(new_host_mem, host_tlb, device_mem, device_tlb)
 
     // The data is unchanged
     ensures host_tlb[vpn].ppn in new_host_mem
@@ -47,6 +63,7 @@ method dma_write(vpn : int,
 
     // We are reading from the device, there should be data there
     requires(vpn_present(vpn, device_mem, device_tlb))
+    requires no_page_aliasing(host_tlb) && no_page_aliasing(device_tlb)
 
 
     // Original host/device pages are untouched
@@ -68,11 +85,28 @@ method write_tlb(vpn : int, ppn : int, present : bool, readable : bool, writable
     returns (new_tlb : map<int, tlb_entry>)
 
     // Old data is unchanged
+    requires no_page_aliasing(tlb)
+
     ensures no_side_effects(vpn, mem, tlb, mem, new_tlb)
     ensures valid_ppns(mem, tlb) && !present ==> valid_ppns(mem, new_tlb)
     ensures valid_ppns(mem, tlb) && present && ppn in mem ==> valid_ppns(mem, new_tlb)
     ensures valid_memory(mem, tlb, other_mem, other_tlb) && !present ==> valid_memory(mem, new_tlb, other_mem, other_tlb)
-    ensures valid_memory(mem, tlb, other_mem, other_tlb) && ppn in mem && !vpn_present(vpn, other_mem, other_tlb) ==> valid_memory(mem, new_tlb, other_mem, other_tlb)
+    ensures valid_memory(mem, tlb, other_mem, other_tlb) && 
+        ppn in mem && !vpn_present(vpn, other_mem, other_tlb) ==> valid_memory(mem, new_tlb, other_mem, other_tlb)
+    ensures valid_memory(mem, tlb, other_mem, other_tlb) && 
+        ppn in mem && 
+        readable && !writable &&
+        ppn_readable(vpn, other_mem, other_tlb) && !ppn_writable(vpn, other_mem, other_tlb) &&
+        mem[ppn] == other_mem[other_tlb[vpn].ppn] ==> valid_memory(mem, new_tlb, other_mem, other_tlb)
+    ensures valid_memory(mem, tlb, other_mem, other_tlb) && 
+        ppn in mem && 
+        readable && !writable &&
+        !ppn_readable(vpn, other_mem, other_tlb) && !ppn_writable(vpn, other_mem, other_tlb)
+        ==> valid_memory(mem, new_tlb, other_mem, other_tlb)
+    // ensures valid_memory(mem, tlb, other_mem, other_tlb) && ppn in mem && !writable && !ppn_writable(vpn, other_mem, other_tlb) ==> valid_memory(mem, new_tlb, other_mem, other_tlb)
+    
+    ensures (vpn in tlb && ppn == tlb[vpn].ppn) ==> no_page_aliasing(new_tlb)
+    ensures (forall vpn :: vpn in tlb ==> tlb[vpn].ppn != ppn) ==> no_page_aliasing(new_tlb)
 
     // actual update takes place
     ensures vpn in new_tlb
@@ -167,9 +201,16 @@ function valid_ppns(mem : map<int, page>, tlb : map<int, tlb_entry>) : bool
 function valid_memory(mem1 : map<int, page>, tlb1 : map<int, tlb_entry>, mem2 : map<int, page>, tlb2 : map<int, tlb_entry>) : bool 
 {
     var ppns_valid := valid_ppns(mem1, tlb1) && valid_ppns(mem2, tlb2);
-    var no_duplicates := forall vpage :: !((vpage in tlb1 && tlb1[vpage].present) && (vpage in tlb2 && tlb2[vpage].present));
+    var no_duplicate_writable_pages := 
+        forall vpn ::
+            !(ppn_writable(vpn, mem1, tlb1) && vpn_present(vpn, mem2, tlb2)) &&
+            !(ppn_writable(vpn, mem2, tlb2) && vpn_present(vpn, mem1, tlb1));
 
-    ppns_valid && no_duplicates
+    var readonly_pages_equal :=
+        forall vpn ::
+            ppn_readable(vpn, mem1, tlb1) && ppn_readable(vpn, mem2, tlb2) ==> mem1[tlb1[vpn].ppn] == mem2[tlb2[vpn].ppn];
+
+    ppns_valid && no_duplicate_writable_pages && readonly_pages_equal
 }
 
 // read from memory on the host
@@ -186,13 +227,14 @@ method read_host(vpn : int,
     // Data must also exist and be readable somewhere
     requires ppn_readable(vpn, host_mem, host_tlb) || ppn_readable(vpn, device_mem, device_tlb)
     requires valid_memory(host_mem, host_tlb, device_mem, device_tlb)
+    requires no_page_aliasing(host_tlb) && no_page_aliasing(device_tlb)
 
     // ensures vpn_present(vpn, new_host_mem, new_host_tlb)
     // The data should reside on the host after executing this method
     ensures ppn_readable(vpn, new_host_mem, new_host_tlb)
 
     // The data should not be accessible on the device after executing this method
-    ensures !vpn_present(vpn, device_mem, new_device_tlb)
+    ensures !ppn_writable(vpn, device_mem, new_device_tlb)
 
     ensures data_unchanged(vpn, host_mem, host_tlb, device_mem, device_tlb, data, new_host_mem, new_host_tlb, device_mem, new_device_tlb)
 
@@ -200,23 +242,23 @@ method read_host(vpn : int,
     ensures no_side_effects(vpn, host_mem, host_tlb, new_host_mem, new_host_tlb)
     ensures no_side_effects(vpn, device_mem, device_tlb, device_mem, new_device_tlb)
 
-    ensures permissions_unchanged(vpn, host_mem, host_tlb, device_mem, device_tlb, new_host_mem, new_host_tlb, device_mem, new_device_tlb)
+    // ensures permissions_unchanged(vpn, host_mem, host_tlb, device_mem, device_tlb, new_host_mem, new_host_tlb, device_mem, new_device_tlb)
     ensures valid_memory(new_host_mem, new_host_tlb, device_mem, new_device_tlb)
+    ensures no_page_aliasing(new_host_tlb) && no_page_aliasing(new_device_tlb)
+
 {
     new_host_mem := host_mem;
     new_host_tlb := host_tlb;
 
     new_device_tlb := device_tlb;
 
-    if vpn !in host_tlb || !host_tlb[vpn].present {
-        new_device_tlb := write_tlb(vpn, 0, false, false, false, device_tlb, device_mem, host_tlb, host_mem);
-        var should_be_writable := device_tlb[vpn].writable;
+    if vpn !in host_tlb || !host_tlb[vpn].present || !host_tlb[vpn].readable {
+        var old_entry := device_tlb[vpn];
+        new_device_tlb := write_tlb(vpn, old_entry.ppn, true, true, false, device_tlb, device_mem, host_tlb, host_mem);
         var curr_entry := host_tlb[vpn];
-        var writeable_host_tlb := host_tlb[vpn := tlb_entry.Node(true, true, true, curr_entry.ppn)];
-        new_host_mem := dma_read(vpn, host_mem, writeable_host_tlb, device_mem, device_tlb);
-        new_host_tlb := write_tlb(vpn, curr_entry.ppn, true, true, should_be_writable, new_host_tlb, new_host_mem, new_device_tlb, device_mem);
+        new_host_mem := dma_read(vpn, host_mem, host_tlb, device_mem, device_tlb);
+        new_host_tlb := write_tlb(vpn, curr_entry.ppn, true, true, false, new_host_tlb, new_host_mem, new_device_tlb, device_mem);
     }
-
     data := new_host_mem[new_host_tlb[vpn].ppn].data;
     return;
 }
@@ -233,6 +275,7 @@ method write_host(vpn : int, data : int,
     // Data must also exist and be readable somewhere
     requires ppn_writable(vpn, host_mem, host_tlb) || ppn_writable(vpn, device_mem, device_tlb)
     requires valid_memory(host_mem, host_tlb, device_mem, device_tlb)
+    requires no_page_aliasing(host_tlb) && no_page_aliasing(device_tlb)
 
     // The data should reside on the host after executing this method
     ensures ppn_writable(vpn, new_host_mem, new_host_tlb)
@@ -251,6 +294,7 @@ method write_host(vpn : int, data : int,
 
     ensures permissions_unchanged(vpn, host_mem, host_tlb, device_mem, device_tlb, new_host_mem, new_host_tlb, device_mem, new_device_tlb)
     ensures valid_memory(new_host_mem, new_host_tlb, device_mem, new_device_tlb)
+    ensures no_page_aliasing(new_host_tlb) && no_page_aliasing(new_device_tlb)
 {
     new_host_mem := host_mem;
     new_host_tlb := host_tlb;
@@ -260,7 +304,7 @@ method write_host(vpn : int, data : int,
 
     if vpn !in host_tlb || !host_tlb[vpn].present {
         var should_be_readable := device_tlb[vpn].readable;
-        new_device_tlb := write_tlb(vpn, 0, false, false, false, device_tlb, device_mem, host_tlb, host_mem);
+        new_device_tlb := write_tlb(vpn, device_tlb[vpn].ppn, false, false, false, device_tlb, device_mem, host_tlb, host_mem);
         var curr_entry := host_tlb[vpn];
         var writeable_host_tlb := host_tlb[vpn := tlb_entry.Node(true, true, true, curr_entry.ppn)];
         new_host_mem := dma_read(vpn, host_mem, writeable_host_tlb, device_mem, device_tlb);
@@ -270,11 +314,17 @@ method write_host(vpn : int, data : int,
     return; 
 }
 
-method allocate_device_ppn(device_mem : map<int, page>)
+method allocate_device_ppn(device_mem : map<int, page>, ghost device_tlb : map<int, tlb_entry>)
     returns (pg : int, new_device_mem : map<int, page>)
+    requires forall ppn :: ppn !in device_mem ==> forall vpn :: vpn in device_tlb ==> device_tlb[vpn].ppn != ppn
+
+    requires no_page_aliasing(device_tlb)
+
     ensures pg !in device_mem
     ensures pg in new_device_mem
     ensures forall p :: p in device_mem ==> p in new_device_mem && device_mem[p] == new_device_mem[p]
+    // forall vpn :: vpn in tlb && tlb[vpn].ppn != ppn
+    ensures forall vpn :: vpn in device_tlb ==> device_tlb[vpn].ppn != pg
 {
     var keys := device_mem.Keys;
     pg := 0;
@@ -304,18 +354,23 @@ method read_device(vpn : int,
             new_host_mem : map<int, page>, new_host_tlb : map<int, tlb_entry>, 
             new_device_mem : map<int, page>, new_device_tlb : map<int, tlb_entry>)
 
+    // The tlb only currently points to pages in memory. this is required to guarantee that the allocator 
+    // doesn't cause any aliasing
+    requires forall ppn :: ppn !in device_mem ==> forall vpn :: vpn in device_tlb ==> device_tlb[vpn].ppn != ppn
+
     // data must exist on the host so that we have a ppn for it
     requires legal_vaddr(vpn, host_mem, host_tlb)
     // Data must also exist and be readable somewhere
     requires ppn_readable(vpn, host_mem, host_tlb) || ppn_readable(vpn, device_mem, device_tlb)
     requires valid_memory(host_mem, host_tlb, device_mem, device_tlb)
+    requires no_page_aliasing(host_tlb) && no_page_aliasing(device_tlb)
 
     // ensures vpn_present(vpn, new_host_mem, new_host_tlb)
     // The data should reside on the device after executing this method
     ensures ppn_readable(vpn, new_device_mem, new_device_tlb)
 
     // The data should not be accessible on the host after executing this method
-    ensures !vpn_present(vpn, new_host_mem, new_host_tlb)
+    ensures !ppn_writable(vpn, new_host_mem, new_host_tlb)
 
     ensures data_unchanged(vpn, host_mem, host_tlb, device_mem, device_tlb, data, new_host_mem, new_host_tlb, new_device_mem, new_device_tlb)
 
@@ -323,8 +378,8 @@ method read_device(vpn : int,
     ensures no_side_effects(vpn, host_mem, host_tlb, new_host_mem, new_host_tlb)
     ensures no_side_effects(vpn, device_mem, device_tlb, device_mem, new_device_tlb)
 
-    ensures permissions_unchanged(vpn, host_mem, host_tlb, device_mem, device_tlb, new_host_mem, new_host_tlb, device_mem, new_device_tlb)
     ensures valid_memory(new_host_mem, new_host_tlb, new_device_mem, new_device_tlb)
+    ensures no_page_aliasing(new_host_tlb) && no_page_aliasing(new_device_tlb)
 {
     new_host_mem := host_mem;
     new_host_tlb := host_tlb;
@@ -332,14 +387,15 @@ method read_device(vpn : int,
     new_device_mem := device_mem;
     new_device_tlb := device_tlb;
 
-    if vpn !in device_tlb || !device_tlb[vpn].present {
+    if vpn !in device_tlb || !device_tlb[vpn].present || !device_tlb[vpn].readable {
         var should_be_writable := host_tlb[vpn].writable;
         var ppn;
-        ppn, new_device_mem := allocate_device_ppn(device_mem);
-        new_host_tlb := write_tlb(vpn, 0, false, false, false, host_tlb, new_host_mem, new_device_tlb, new_device_mem);
+        ppn, new_device_mem := allocate_device_ppn(device_mem, device_tlb);
+
+        new_host_tlb := write_tlb(vpn, host_tlb[vpn].ppn, false, false, false, host_tlb, new_host_mem, new_device_tlb, new_device_mem);
         new_device_tlb := write_tlb(vpn, ppn, true, true, should_be_writable, new_device_tlb, new_device_mem, new_host_tlb, new_host_mem);
         new_device_mem := dma_write(vpn, host_mem, host_tlb, new_device_mem, new_device_tlb);
-    } 
+    }
     data := new_device_mem[new_device_tlb[vpn].ppn].data;
     return;
 }
@@ -387,7 +443,7 @@ method write_device(vpn : int, data : int,
     if vpn !in device_tlb || !device_tlb[vpn].present {
         var should_be_readable := host_tlb[vpn].readable;
         var ppn;
-        ppn, new_device_mem := allocate_device_ppn(device_mem);
+        ppn, new_device_mem := allocate_device_ppn(device_mem, device_tlb);
         new_host_tlb := write_tlb(vpn, 0, false, false, false, host_tlb, new_host_mem, new_device_tlb, new_device_mem);
         new_device_tlb := write_tlb(vpn, ppn, true, should_be_readable, true, new_device_tlb, new_device_mem, new_host_tlb, new_host_mem);
         new_device_mem := dma_write(vpn, host_mem, host_tlb, new_device_mem, new_device_tlb);
